Make simulation definition to account for future programs of the current module.

common/Linkeq.v
@@ -3,7 +3,7 @@ Require String.
 Require Import Coqlib Coqlib_linker.
 Require Import Maps_linker.
 Require Import Integers Floats Values AST Globalenvs.
-Require Import LinkerSpecification.
+Require Import LinkerSpecification LinkerProp.
 
 Set Implicit Arguments.
 
@@ -13,6 +13,8 @@ Section Linkeq.
 
 Variable (Fundef F EF V:Type).
 Variable (fundef_dec: FundefDec Fundef F EF).
+Variable (EF_dec: forall (v1 v2:EF), {v1 = v2} + {v1 <> v2}).
+Variable (V_dec: forall (v1 v2:V), {v1 = v2} + {v1 <> v2}).
 
 (** `linkeq a b` means `b` is a possible future global definition of `a` after linkings *)
 
@@ -32,16 +34,23 @@ Inductive globdef_linkeq: forall (g1 g2:globdef Fundef V), Prop :=
     globdef_linkeq (Gvar v1) (Gvar v2)
 .
 
-Definition globaldefs_linkeq (defs1 defs2:PTree.t (globdef Fundef V)): Prop :=
+Definition globdefs_linkeq (defs1 defs2:PTree.t (globdef Fundef V)): Prop :=
   forall var def1 (Hsrc: PTree.get var defs1 = Some def1),
   exists def2,
     PTree.get var defs2 = Some def2 /\
     globdef_linkeq def1 def2.
 
+Definition globdef_list_linkeq (defs1 defs2:list (positive * globdef Fundef V)): Prop :=
+  globdefs_linkeq (PTree.unelements defs1) (PTree.unelements defs2).
 
-(** `linkable` and `linkeq` properties *)
+Definition program_linkeq (p1 p2:program Fundef V): Prop :=
+  globdef_list_linkeq p1.(prog_defs) p2.(prog_defs) /\
+  p1.(prog_main) = p2.(prog_main).
 
-Program Instance globfun_linkeq_PreOrder: PreOrder globfun_linkeq.
+
+(** preorders *)
+
+Global Program Instance globfun_linkeq_PreOrder: PreOrder globfun_linkeq.
 Next Obligation.
   intro f. left. auto.
 Qed.
@@ -56,16 +65,7 @@ Next Obligation.
   - right. eapply globfun_linkable_ee; eauto.
 Qed.
 
-Lemma globdef_linkable_linkeq
-      g1 g2 (Hlinkable: globdef_linkable fundef_dec g1 g2):
-  globdef_linkeq g1 g2.
-Proof.
-  inv Hlinkable; constructor; auto.
-  - right. auto.
-  - right. auto.
-Qed.
-
-Program Instance globvar_linkeq_PreOrder: PreOrder globvar_linkeq.
+Global Program Instance globvar_linkeq_PreOrder: PreOrder globvar_linkeq.
 Next Obligation.
   intros [info init readonly volatile].
   constructor; auto.
@@ -84,7 +84,7 @@ Next Obligation.
   - rewrite Hvolatile. auto.
 Qed.
 
-Program Instance globdef_linkeq_PreOrder: PreOrder globdef_linkeq.
+Global Program Instance globdef_linkeq_PreOrder: PreOrder globdef_linkeq.
 Next Obligation.
   intros [f|v]; constructor; reflexivity.
 Qed.
@@ -92,6 +92,146 @@ Next Obligation.
   intros [f1|v1] [f2|v2] [f3|v3] H12 H23; inv H12; inv H23.
   - constructor. rewrite Hv. auto.
   - constructor. rewrite Hv. auto.
+Qed.
+
+Global Program Instance globdefs_linkeq_PreOrder: PreOrder globdefs_linkeq.
+Next Obligation.
+  repeat intro. eexists. split; eauto. reflexivity.
+Qed.
+Next Obligation.
+  repeat intro.
+  exploit H; eauto. intros [ydef [Hydef Hxy]].
+  exploit H0; eauto. intros [zdef [Hzdef Hyz]].
+  eexists. split; eauto. rewrite Hxy. auto.
+Qed.
+
+Global Program Instance globdef_list_linkeq_PreOrder: PreOrder globdef_list_linkeq.
+Next Obligation.
+  repeat intro. eexists. split; eauto. reflexivity.
+Qed.
+Next Obligation.
+  intros x y z Hxy Hyz. unfold globdef_list_linkeq in *.
+  rewrite Hxy. auto.
+Qed.
+
+Global Program Instance program_linkeq_PreOrder: PreOrder program_linkeq.
+Next Obligation.
+  repeat intro. split; reflexivity.
+Qed.
+Next Obligation.
+  intros x y z [Hxy_defs Hxy_main] [Hyz_defs Hyz_main].
+  split.
+  - rewrite Hxy_defs. auto.
+  - rewrite Hxy_main. auto.
+Qed.
+
+
+(** `linkable` and `linkeq` properties *)
+
+Lemma globdef_linkable_linkeq
+      g1 g2 (Hlinkable: globdef_linkable fundef_dec g1 g2):
+  globdef_linkeq g1 g2.
+Proof.
+  inv Hlinkable; constructor; auto.
+  - right. auto.
+  - right. auto.
+Qed.
+
+
+(** properties of linking on linkeq *)
+
+Lemma link_globdefs_linkeq_l
+      defs1 defs2 defs
+      (Hdefs: link_globdefs fundef_dec EF_dec V_dec defs1 defs2 = Some defs):
+  globdefs_linkeq defs1 defs.
+Proof.
+  repeat intro.
+  exploit gtlink_globdefs; eauto. instantiate (1 := var). rewrite Hsrc.
+  destruct (defs2 ! var) as [def2|], (defs ! var) as [def|]; intro X; inv X.
+  - destruct H. subst. eexists. split; eauto.
+    apply globdef_linkable_linkeq. auto.
+  - destruct H. subst. eexists. split; eauto.
+    reflexivity.
+  - eexists. split; eauto.
+    reflexivity.
+Qed.
+
+Lemma link_globdefs_linkeq_r
+      defs1 defs2 defs
+      (Hdefs: link_globdefs fundef_dec EF_dec V_dec defs1 defs2 = Some defs):
+  globdefs_linkeq defs2 defs.
+Proof.
+  repeat intro.
+  exploit gtlink_globdefs; eauto. instantiate (1 := var). rewrite Hsrc.
+  destruct (defs1 ! var) as [d1|], (defs ! var) as [d|]; intro X; inv X.
+  - destruct H. subst. eexists. split; eauto.
+    reflexivity.
+  - destruct H. subst. eexists. split; eauto.
+    apply globdef_linkable_linkeq. auto.
+  - eexists. split; eauto.
+    reflexivity.
+Qed.
+
+Lemma link_globdef_list_linkeq_l
+      defs1 defs2 defs
+      (Hdefs: link_globdef_list fundef_dec EF_dec V_dec defs1 defs2 = Some defs):
+  globdef_list_linkeq defs1 defs.
+Proof.
+  unfold globdef_list_linkeq, link_globdef_list in *.
+  match goal with
+    | [H: context[link_globdefs ?fundef_dec ?EF_dec ?V_dec ?defs1 ?defs2] |- _] =>
+      destruct (link_globdefs fundef_dec EF_dec V_dec defs1 defs2) as [defs'|] eqn:Hdefs'; inv H
+  end.
+  admit. (* TODO: PTree.elements, PTree.unelements *)
+Qed.
+
+Lemma link_globdef_list_linkeq_r
+      defs1 defs2 defs
+      (Hdefs: link_globdef_list fundef_dec EF_dec V_dec defs1 defs2 = Some defs):
+  globdef_list_linkeq defs2 defs.
+Proof.
+  unfold globdef_list_linkeq, link_globdef_list in *.
+  match goal with
+    | [H: context[link_globdefs ?fundef_dec ?EF_dec ?V_dec ?defs1 ?defs2] |- _] =>
+      destruct (link_globdefs fundef_dec EF_dec V_dec defs1 defs2) as [defs'|] eqn:Hdefs'; inv H
+  end.
+  admit. (* TODO: PTree.elements, PTree.unelements *)
+Qed.
+
+Lemma link_program_linkeq_l
+      p1 p2 p (Hp: link_program fundef_dec EF_dec V_dec p1 p2 = Some p):
+  program_linkeq p1 p.
+Proof.
+  destruct p1 as [defs1 main1].
+  destruct p2 as [defs2 main2].
+  destruct p as [defs main].
+  unfold link_program in Hp. simpl in *.
+  destruct ((main1 =? main2)%positive) eqn:Hmain; inv Hp.
+  apply Pos.eqb_eq in Hmain. subst.
+  match goal with
+    | [H: context[link_globdef_list ?fundef_dec ?EF_dec ?V_dec ?defs1 ?defs2] |- _] =>
+      destruct (link_globdef_list fundef_dec EF_dec V_dec defs1 defs2) as [defs'|] eqn:Hdefs'; inv H
+  end.
+  split; simpl; auto.
+  eapply link_globdef_list_linkeq_l. eauto.
+Qed.
+
+Lemma link_program_linkeq_r
+      p1 p2 p (Hp: link_program fundef_dec EF_dec V_dec p1 p2 = Some p):
+  program_linkeq p2 p.
+Proof.
+  destruct p1 as [defs1 main1].
+  destruct p2 as [defs2 main2].
+  destruct p as [defs main].
+  unfold link_program in Hp. simpl in *.
+  destruct ((main1 =? main2)%positive) eqn:Hmain; inv Hp.
+  apply Pos.eqb_eq in Hmain. subst.
+  match goal with
+    | [H: context[link_globdef_list ?fundef_dec ?EF_dec ?V_dec ?defs1 ?defs2] |- _] =>
+      destruct (link_globdef_list fundef_dec EF_dec V_dec defs1 defs2) as [defs'|] eqn:Hdefs'; inv H
+  end.
+  split; simpl; auto.
+  eapply link_globdef_list_linkeq_r. eauto.
 Qed.
 
 End Linkeq.
