common/LinkerProp.v
@@ -1,0 +1,71 @@
+Require Import RelationClasses.
+Require String.
+Require Import Coqlib Coqlib_linker.
+Require Import Maps_linker.
+Require Import Integers Floats Values AST Globalenvs.
+Require Import LinkerSpecification.
+Require Import Errors.
+
+Set Implicit Arguments.
+
+Section LINKER_PROP.
+
+Variable (Fundef F EF V:Type).
+Variable (fundef_dec: FundefDec Fundef F EF).
+Variable (EF_dec: forall (v1 v2:EF), {v1 = v2} + {v1 <> v2}).
+Variable (V_dec: forall (v1 v2:V), {v1 = v2} + {v1 <> v2}).
+
+Lemma gflink_globdefs defs1 defs2 (Hlink: link_globdefs fundef_dec EF_dec V_dec defs1 defs2 = None):
+  exists var def1 def2,
+    PTree.get var defs1 = Some def1 /\
+    PTree.get var defs2 = Some def2 /\
+    ~ globdef_linkable fundef_dec def1 def2 /\
+    ~ globdef_linkable fundef_dec def2 def1.
+Proof.
+  unfold link_globdefs in Hlink.
+  match goal with
+    | [H: context[PTree_Properties.for_all ?m ?f] |- _] =>
+      destruct (PTree_Properties.for_all m f) eqn:Hlinkable; inv Hlink
+  end.
+  apply PTree_Properties.for_all_false in Hlinkable.
+  destruct Hlinkable as [i [x [Hx1 Hx2]]].
+  destruct x; inv Hx2. rewrite PTree.gcombine in Hx1; auto.
+  destruct (defs1 ! i) eqn:Hi1, (defs2 ! i) eqn:Hi2; inv Hx1.
+  destruct (globdef_linkable_dec fundef_dec EF_dec V_dec g g0); inv H0.
+  destruct (globdef_linkable_dec fundef_dec EF_dec V_dec g0 g); inv H1.
+  repeat eexists; eauto.
+Qed.
+
+Lemma gtlink_globdefs defs1 defs2 defs (Hlink: link_globdefs fundef_dec EF_dec V_dec defs1 defs2 = Some defs):
+  forall var,
+    match PTree.get var defs1, PTree.get var defs2, PTree.get var defs with
+      | Some g1, Some g2, Some g =>
+        (globdef_linkable fundef_dec g1 g2 /\ g2 = g) \/
+        (globdef_linkable fundef_dec g2 g1 /\ g1 = g)
+      | Some g1, None, Some g => g1 = g
+      | None, Some g2, Some g => g2 = g
+      | None, None, None => True
+      | _, _, _ => False
+    end.
+Proof.
+  intro i. unfold link_globdefs in Hlink.
+  match goal with
+    | [H: context[PTree_Properties.for_all ?m ?f] |- _] =>
+      destruct (PTree_Properties.for_all m f) eqn:Hlinkable; inv Hlink
+  end.
+  rewrite PTree.goption_map, PTree.gcombine; auto.
+  destruct (defs1 ! i) eqn:Hi1, (defs2 ! i) eqn:Hi2; auto.
+  destruct (globdef_linkable_dec fundef_dec EF_dec V_dec g g0).
+  { left. split; auto. }
+  destruct (globdef_linkable_dec fundef_dec EF_dec V_dec g0 g).
+  { right. split; auto. }
+  eapply PTree_Properties.for_all_correct in Hlinkable; eauto.
+  { instantiate (1 := None) in Hlinkable. inv Hlinkable. }
+  instantiate (1 := i). rewrite PTree.gcombine; auto.
+  rewrite Hi1, Hi2.
+  destruct (globdef_linkable_dec fundef_dec EF_dec V_dec g g0); try (contradict n; auto; fail).
+  destruct (globdef_linkable_dec fundef_dec EF_dec V_dec g0 g); try (contradict n0; auto; fail).
+  auto.
+Qed.
+
+End LINKER_PROP.
